CredibleCompilation/CSEOptExamples.lean
@@ -26,7 +26,7 @@ namespace CSEOptExamples
     2: halt
 -/
 
-def simpleProg : Prog := #[
+def simpleProg : Prog := .ofCode #[
   .binop "a" .add "x" "y",
   .binop "b" .add "x" "y",
   .halt
@@ -57,7 +57,7 @@ def simpleCert := optimize simpleProg ("b" :: [])
     4: halt
 -/
 
-def chainProg : Prog := #[
+def chainProg : Prog := .ofCode #[
   .binop "a" .add "x" "y",
   .binop "b" .add "a" "z",
   .binop "c" .add "x" "y",
@@ -84,7 +84,7 @@ def chainCert := optimize chainProg ("c" :: "d" :: [])
   Expected: no optimization (expression killed)
 -/
 
-def killProg : Prog := #[
+def killProg : Prog := .ofCode #[
   .binop "a" .add "x" "y",
   .const "x" (.int 42),
   .binop "b" .add "x" "y",
@@ -109,7 +109,7 @@ def killCert := optimize killProg ("b" :: [])
     4: halt
 -/
 
-def multiProg : Prog := #[
+def multiProg : Prog := .ofCode #[
   .binop "a" .add "x" "y",
   .binop "b" .mul "x" "y",
   .binop "c" .add "x" "y",
@@ -138,7 +138,7 @@ def multiCert := optimize multiProg ("c" :: "d" :: [])
   Expected: pc 4 becomes copy c a
 -/
 
-def constProg : Prog := #[
+def constProg : Prog := .ofCode #[
   .const "x" (.int 5),
   .const "y" (.int 3),
   .binop "a" .add "x" "y",
@@ -168,7 +168,7 @@ def constCert := optimize constProg ("c" :: [])
   available through the loop back-edge.
 -/
 
-def loopProg : Prog := #[
+def loopProg : Prog := .ofCode #[
   .binop "a" .add "x" "y",
   .ifgoto (.cmpLit .lt "a" 100) 3,
   .halt,
@@ -194,7 +194,7 @@ def loopCert := optimize loopProg ("b" :: [])
   Expected: no optimization (x was overwritten)
 -/
 
-def aliasProg : Prog := #[
+def aliasProg : Prog := .ofCode #[
   .binop "x" .add "x" "y",
   .binop "a" .add "x" "y",
   .halt
